@prefix schema: <https://schema.org/> .
@prefix rdf: <http://www.w3.org/1999/02/22-rdf-syntax-ns#> .
@prefix rdfs: <http://www.w3.org/2000/01/rdf-schema#>.
@prefix owl: <http://www.w3.org/2002/07/owl#>.
@prefix spv: <https://bmake.th-brandenburg.de/spv#>.
@prefix skos: <http://www.w3.org/2004/02/skos/core#>.
@prefix xsd: <http://www.w3.org/2001/XMLSchema#>.
@prefix spe: <https://bmake.th-brandenburg.de/spe#> .
@prefix wd: <http://www.wikidata.org/entity/>.


### Class Definitions ###
schema:CreativeWork a owl:Class ;
			rdfs:label "Creative Work" ;
			rdfs:comment "Here used primarily for scientific papers, conference proceeding and related creative work." .
			
schema:ScholarlyArticle a owl:Class ;
			rdfs:label "Scholarly Article" ;
			rdfs:subClassOf schema:CreativeWork ;
			rdfs:comment "The class of scientific papers." .
			
schema:CreativeWorkSeries a owl:Class ;
			rdfs:label "Creative Work Series" ;
			rdfs:subClassOf schema:CreativeWork ;
			rdfs:comment "The class of Conference proceedings - independent of the publication format." .
			
schema:Event a owl:Class ;
			rdfs:label "Event" ;
			rdfs:comment "Here used primarily for scientific conferences." .
			
schema:PublicationEvent a owl:Class ;
			rdfs:label "Publication Event" ;
			rdfs:subClassOf schema:Event ;
			rdfs:comment "The class of scientific conferences." .
			
schema:Organization a owl:Class ;
			rdfs:label "Organization" ;
			rdfs:comment "Here used for two objectives: (i) to denote the affiliations of authors and other Person and (ii) for indicate publishers and conference organizers." .
			
schema:Place a owl:Class ;
			rdfs:label "Place" ;
			rdfs:comment "Here used for specifying the locations of conferences and organizations." .
			
schema:Person a owl:Class ;
			rdfs:label "Person" ;
			rdfs:comment "Mainly used for identifying authors, editors, attendees, contributers, organizers and other human agents." .
				
schema:Intangible a owl:Class ;
			rdfs:label "Inangible" ;
			rdfs:comment "A utility class that serves as the umbrella for a number of 'intangible' things such as quantities, structured values, etc. (taken from schema.org)." .
			
schema:Enumeration a owl:Class ;
			rdfs:label "Enumeration" ;
			rdfs:comment  "Lists or enumerations of aspects specifying a scientific paper, like research methods, research artifacts and research action types." ;
			rdfs:subClassOf schema:Intangible .
			
schema:StructuredValue a owl:Class ;
			rdfs:label "Structured Value" ;
			rdfs:comment  "Structured values are used when the value of a property has a more complex structure than simply being a textual value or a reference to another thing. Here used for specifying research objectives characterized by research actions applied to research artifacts." ;
			rdfs:subClassOf schema:Intangible .
			
schema:ItemList a owl:Class ;
			rdfs:label "Item List" ;
			rdfs:comment  "Lists of enumerations of aspects specifying a scientific paper, like research methods, research findings, research objectives, and future work." ;
			rdfs:subClassOf schema:Intangible .
					
spv:ResearchMethod a owl:Class ;
			rdfs:label "Research Method" ;
			rdfs:comment "List of all relevant research methods used in Information Systems." ;
			rdfs:subClassOf schema:Enumeration .
					
spv:ResearchArtifact a owl:Class ;
			rdfs:label "Research Artifact" ;
			rdfs:comment "Classification of all types of research & development artifacts characteristic for Information Systems." ;
			rdfs:subClassOf schema:Enumeration .
					
spv:ResearchActionType a owl:Class ;
			rdfs:label "Research Action Type" ;
			rdfs:comment "Classification of all types of research & development actions applied in Information Systems." ;
			rdfs:subClassOf schema:Enumeration .
					
schema:Language a owl:Class ;
			rdfs:label "Language" ;
			rdfs:comment "Natural languages such as Spanish, Tamil, Hindi, English, etc." ;
			rdfs:subClassOf schema:Intangible .
			
schema:DataType a rdfs:Class ;
			rdfs:label "Data Type" ;
			rdfs:comment "Encompasses basic data types for typing literals. ".

schema:Text a rdfs:Class ;
			rdfs:label "Data Type" ;
			rdfs:comment "General class for all literals being of any textual Datatype." ;
			rdfs:subClassOf schema:DataType .
			
schema:URL a rdfs:Class ;
			rdfs:label "URL" ;
			rdfs:comment "General class for all literals being an URL." ;
			rdfs:subClassOf schema:Text .

schema:DateTime a rdfs:Class ;
			rdfs:label "Date and Time" ;
			rdfs:comment "General class for all literals indicating a data and a time." ;
			rdfs:subClassOf schema:DataType .
			
schema:Date a rdfs:Class ;
			rdfs:label "Date" ;
			rdfs:comment "General class for all literals indicating a data." ;
			rdfs:subClassOf schema:DataType .
			
			
### Object properties ###
schema:about a owl:ObjectProperty ;
			rdfs:label "about" ;
			rdfs:comment "Is used to relate to subject matters of a creative work, mainly a scientific paper. Here mainly used to relate to blank nodes of type schema:ItemList for specifying characteristics of a scientific paper, like research findings, research methods and research objectives." ;
			rdfs:domain schema:CreativeWork ;
			rdfs:range owl:Thing .
			
schema:citation a owl:ObjectProperty ;
			rdfs:label "citation" ;
			rdfs:comment "Is used to create references of a scientific paper to other items of creative work (particularly other papers)." ;
			rdfs:domain schema:ScholarlyArticle ;
			rdfs:range xsd:string .
			
schema:isPartOf a owl:ObjectProperty ;
			rdfs:label "is part of" ;
			rdfs:comment "Is used to indicate the proceedings where a scientific paper is published." ;
			rdfs:domain schema:ScholarlyArticle ;
			rdfs:range schema:CreativeWorkSeries .
			
schema:author a owl:ObjectProperty ;
			rdfs:label "author" ;
			rdfs:comment "Is used to indicate a author of a scientific paper." ;
			rdfs:domain schema:ScholarlyArticle ;
			rdfs:range schema:Person .
			
schema:affiliation a owl:ObjectProperty ;
			rdfs:label "affiliation" ;
			rdfs:comment "Is used to indicate the affiliation of a person to an organization." ;
			rdfs:domain schema:Person ;
			rdfs:range schema:Organization .
			
schema:editor a owl:ObjectProperty ;
			rdfs:label "editor" ;
			rdfs:comment "Is used to indicate an editor of a scientific paper or conference proceedings." ;
			rdfs:domain schema:CreativeWork ;
			rdfs:range schema:Person .
			
schema:publisher a owl:ObjectProperty ;
			rdfs:label "publisher" ;
			rdfs:comment "Is used to indicate a publishing organization of a scientific paper or conference proceedings." ;
			rdfs:domain schema:CreativeWork ;
			rdfs:range schema:Organization .
			
schema:attendee a owl:ObjectProperty ;
			rdfs:label "attendee" ;
			rdfs:comment "Is used to indicate a person attending a conference." ;
			rdfs:domain schema:PublicationEvent ;
			rdfs:range schema:Person .
			
schema:contributor a owl:ObjectProperty ;
			rdfs:label "contributor" ;
			rdfs:comment "Is used to indicate a person contributing to a conference." ;
			rdfs:domain schema:PublicationEvent ;
			rdfs:range schema:Person .
			
schema:organizer a owl:ObjectProperty ;
			rdfs:label "organizer" ;
			rdfs:comment "Is used to indicate a person or an organization organizing a conference." ;
			rdfs:domain schema:PublicationEvent ;
			rdfs:range [owl:unionOf (schema:Person schema:Organization)].
									
schema:recordedIn a owl:ObjectProperty ;
			rdfs:label "recorded in" ;
			rdfs:comment "Is used to relate a conference to the corresponding proceedings." ;
			rdfs:domain schema:PublicationEvent ;
			rdfs:range schema:CreativeWorkSeries .
		
schema:location a owl:ObjectProperty ;
			rdfs:label "location" ;
			rdfs:comment "Is used for different purposes to referring to a geographical place, e. g. for event locations (termporal) or for organization locations (permanent)." ;
			rdfs:domain [owl:unionOf (schema:Organization schema:Event)] ;
			rdfs:range schema:Place .	

schema:itemListElement a rdf:Property ;
			rdfs:label "item list element" ;
  			rdfs:comment "For itemListElement values simple strings or existing entities can be used." ;
  			rdfs:domain schema:ItemList ;
  			rdfs:range [rdf:type owl:Class ; owl:unionOf (xsd:string owl:Thing )] .
  			
spv:researchArtifact a owl:ObjectProperty ;
			rdfs:label "research artifact" ;
			rdfs:comment "Is used in combination with research action type to indicate a research objective of a scientific paper." ;
			rdfs:domain schema:StructuredValue ;
			rdfs:range spv:ResearchArtifact .
			
spv:researchActionType a owl:ObjectProperty ;
			rdfs:label "research action type" ;
			rdfs:comment "Is used in combination with research action type to indicate a research objective of a scientific paper." ;
			rdfs:domain schema:StructuredValue ;
			rdfs:range spv:ResearchActionType .
			
spv:researchMethod a owl:ObjectProperty ;
			rdfs:label "research method" ;
			rdfs:comment "Is used to indicate a research method described in a scientific paper." ;
			rdfs:domain schema:StructuredValue ;
			rdfs:range spv:ResearchMethod .


### Datatype Properties ###
schema:description a owl:DatatypeProperty ;
			rdfs:label "description" ;
			rdfs:comment "General datatype property, potentially usable for description of all resources." ;
			rdfs:range schema:Text .
			
schema:image a owl:DatatypeProperty ;
			rdfs:label "image" ;
			rdfs:comment "General datatype property, potentially usable for relating an image of a resource." ;
			rdfs:range schema:URL .
			
schema:sameAs a owl:DatatypeProperty ;
			rdfs:label "same as" ;
			rdfs:comment "General datatype property, potentially usable for relating one resource to a URL representing the same resource." ;
			rdfs:range schema:URL .

schema:name a owl:DatatypeProperty ;
			rdfs:label "name" ;
			rdfs:comment "General datatype property, potentially usable for specifying the name of a resource." ;
			rdfs:range schema:Text .
			
schema:alternateName a owl:DatatypeProperty ;
			rdfs:label "alternative name" ;
			rdfs:comment "General datatype property, potentially usable for specifying alternative names of a resource." ;
			rdfs:range schema:Text .
			
schema:url a owl:ObjectProperty ;
			rdfs:label "url" ;
			rdfs:comment "General datatype property, potentially usable for specifying the URL of a resource." ;
			rdfs:range schema:URL .

schema:endTime a owl:DatatypeProperty ;
			rdfs:label "end time" ;
			rdfs:comment "The end time of some event." ;
			rdfs:domain schema:Event ;
			rdfs:range schema:DateTime .

schema:startTime a owl:DatatypeProperty ;
			rdfs:label "start time" ;
			rdfs:comment "The start time of some event." ;
			rdfs:domain schema:Event ;
			rdfs:range schema:DateTime .

schema:headline a owl:DatatypeProperty ;
			rdfs:label "headline" ;
			rdfs:comment "Headline of a scientific paper." ;
			rdfs:domain schema:ScholarlyArticle ;
			rdfs:range schema:Text .
			
schema:alternativeHeadline a owl:DatatypeProperty ;
			rdfs:label "alternative headline" ;
			rdfs:comment "A secondary title of a scientific paper." ;
			rdfs:domain schema:ScholarlyArticle ;
			rdfs:range schema:Text .

schema:inLanguage a owl:DatatypeProperty ;
			rdfs:label "in language" ;
			rdfs:comment "The language of the content or performance or used in an event." ;
			rdfs:domain [owl:unionOf (schema:Event schema:CreativeWork) ] ;
			rdfs:range schema:Language .
			
schema:dateCreated a owl:DatatypeProperty ;
			rdfs:label "date created" ;
			rdfs:comment "The date on which the CreativeWork was created or the item was added to a DataFeed." ;
			rdfs:domain schema:CreativeWork ;
			rdfs:range schema:Date .
			
schema:dateModified a owl:DatatypeProperty ;
			rdfs:label "date modified" ;
			rdfs:comment "The date on which the CreativeWork was modified or the item's entry was modified within a DataFeed." ;
			rdfs:domain schema:CreativeWork ;
			rdfs:range schema:Date .	

schema:pageEnd a owl:DatatypeProperty ;
  			rdfs:label "end page" ;
  			rdfs:comment "The page on which the scientific paper ends." ;
  			rdfs:domain schema:ScholarlyArticle ;
  			rdfs:range xsd:string .

schema:pageStart a owl:DatatypeProperty ;
  			rdfs:label "start page" ;
  			rdfs:comment "The page on which the scientific paper starts." ;
  			rdfs:domain schema:ScholarlyArticle ;
  			rdfs:range xsd:string .
			
schema:keywords a owl:DatatypeProperty ;
			rdfs:label "keywords" ;
			rdfs:comment "Keywords or tags used to describe the content of a creative work. Multiple entries in a keywords list are typically delimited by commas." ;
			rdfs:domain schema:CreativeWork ;
			rdfs:range schema:Text .
			
schema:text a owl:DatatypeProperty ;
			rdfs:label "text" ;
			rdfs:comment "The textual content of this creative work." ;
			rdfs:domain schema:CreativeWork ;
			rdfs:range schema:Text .
			
schema:award a owl:DatatypeProperty ;
			rdfs:label "award" ;
			rdfs:comment "An award won by or for this scientific paper." ;
			rdfs:domain schema:ScholarlyArticle ;
			rdfs:range schema:Text .
			
schema:familyName a owl:DatatypeProperty ;
			rdfs:label "family name" ;
			rdfs:comment "The last name of a Person." ;
			rdfs:domain schema:Person ;
			rdfs:range schema:Text .
			
schema:givenName a owl:DatatypeProperty ;
			rdfs:label "given name" ;
			rdfs:comment "The first name of a Person." ;
			rdfs:domain schema:Person ;
			rdfs:range schema:Text .			
				
schema:additionalName a owl:DatatypeProperty ;
			rdfs:label "additional name" ;
			rdfs:comment "The additional name for Person, can be used for a middle name." ;
			rdfs:domain schema:Person ;
			rdfs:range schema:Text .

schema:honoricPrefix a owl:DatatypeProperty ;
			rdfs:label "honoric prefix" ;
			rdfs:comment "An honorific prefix preceding a Person's name such as Dr/Mrs/Mr." ;
			rdfs:domain schema:Person ;
			rdfs:range schema:Text .

schema:honoricSuffix a owl:DatatypeProperty ;
			rdfs:label "honoric suffix" ;
			rdfs:comment "An honorific suffix preceding a Person's name such as M.D. /PhD/MSCSW." ;
			rdfs:domain schema:Person ;
			rdfs:range schema:Text .

schema:jobTitle a owl:DatatypeProperty ;
			rdfs:label "job title" ;
			rdfs:comment "The job title of the person (for example, Knowledge Engineer)." ;
			rdfs:domain schema:Person ;
			rdfs:range schema:Text .
			
schema:email a owl:DatatypeProperty ;
			rdfs:label "email" ;
			rdfs:comment "Email address of a person or an organization." ;
			rdfs:domain [owl:unionOf (schema:Person schema:Organization)] ;
			rdfs:range schema:Text .

schema:telephone a owl:DatatypeProperty ;
			rdfs:label "telephone" ;
			rdfs:comment "Telephone number of a person or an organization." ;
			rdfs:domain [owl:unionOf (schema:Person schema:Organization)] ;
			rdfs:range schema:Text .

schema:faxNumber a owl:DatatypeProperty ;
			rdfs:label "fax number" ;
			rdfs:comment "Fax number of a person or an organization." ;
			rdfs:domain [owl:unionOf (schema:Person schema:Organization)] ;
			rdfs:range schema:Text .

schema:legalName a owl:DatatypeProperty ;
			rdfs:label "legal name" ;
			rdfs:comment "The legal name of an Organization." ;
			rdfs:domain schema:Organization ;
			rdfs:range schema:Text .

schema:logo a owl:DatatypeProperty ;
			rdfs:label "logo" ;
			rdfs:comment "An associated logo of an Organization." ;
			rdfs:domain schema:Organization ;
			rdfs:range schema:URL .
			
			
### Named Individuals ###
## Scientific Methods ##
spv:ResMethDesignScience a owl:NamedIndividual , spv:ResearchMethod ;
			schema:name "Design Science (Hevner)"@en ;
			schema:isBasedOn <http://doi.org/10.1007/978-1-4419-5653-8_2> ;
			rdfs:comment "Description" .
			
spv:ResMethFormalDedAnalysis a owl:NamedIndividual , spv:ResearchMethod ;
			schema:name "Formal Deductive Analysis (Wilde/Hess)"@en ;
			schema:name "Formal-deduktive Analyse (Wilde/Hess)"@de ;
			schema:isBasedOn <http://doi.org/10.1007/s11576-007-0064-z> ;
			rdfs:comment "Logisch-deduktives Schließen im Rahmen mathematisch-formaler Modelle"@de .			

spv:ResMethConceptualDedAnalysis a owl:NamedIndividual , spv:ResearchMethod ;
			schema:name "Conceptual Deductive Analysis (Wilde/Hess)"@en ;
			schema:name "Konzeptionell-deduktive Analyse (Wilde/Hess)"@de ;
			schema:isBasedOn <http://doi.org/10.1007/s11576-007-0064-z> ;
			rdfs:comment "Logisch-deduktives Schließen im Rahmen semiformaler Modelle (z. B. BPMN)."@de .			

spv:ResMethArgumentDedAnalysis a owl:NamedIndividual , spv:ResearchMethod ;
			schema:name "Argumentative Deductive Analysis (Wilde/Hess)"@en ;
			schema:name "Argumentativ-deduktive Analyse (Wilde/Hess)"@de ;
			schema:isBasedOn <http://doi.org/10.1007/s11576-007-0064-z> ;
			rdfs:comment "Rein sprachliches logisch-deduktives Schließen (wie z. B. in der Philosophie)"@de .			

spv:ResMethSimulation a owl:NamedIndividual , spv:ResearchMethod ;
			schema:name "Simulation (Wilde/Hess)"@en ;
			schema:name "Simulation (Wilde/Hess)"@de ;
			schema:isBasedOn <http://doi.org/10.1007/s11576-007-0064-z> ;
			rdfs:comment "Die Simulation bildet das Verhalten des zu untersuchenden Systems formal in einem Modell ab und stellt Umweltzustände durch bestimmte Belegungen der Modellparameter nach. Sowohl durch die Modellkonstruktion als auch durch die Beobachtung der endogenen Modellgrößen lassen sich Erkenntnisse gewinnen."@de .	

spv:ResMethReferenceModeling a owl:NamedIndividual , spv:ResearchMethod ;
			schema:name "Reference Modeling (Wilde/Hess)"@en ;
			schema:name "Reference Modeling (Wilde/Hess)"@de ;
			schema:isBasedOn <http://doi.org/10.1007/s11576-007-0064-z> ;
			rdfs:comment "Die Referenzmodellierung erstellt induktiv (ausgehend von Beobachtungen) oder deduktiv (bspw. aus Theorien oder Modellen) meist vereinfachte und optimierte Abbildungen (Idealkonzepte) von Systemen, um so bestehende Erkenntnisse zu vertiefen und daraus Gestaltungsvorlagen zu generieren"@de .	

spv:ResMethActionResearch a owl:NamedIndividual , spv:ResearchMethod ;
			schema:name "Action Research (Wilde/Hess)"@en ;
			schema:name "Aktionsforschung (Wilde/Hess)"@de ;
			schema:isBasedOn <http://doi.org/10.1007/s11576-007-0064-z> ;
			rdfs:comment "Es wird ein Praxisproblem durch einen gemischten Kreis aus Wissenschaft und Praxis gelöst. Hierbei werden mehrere Zyklen aus Analyse-, Aktions-, und Evaluationsschritten durchlaufen, die jeweils gering strukturierte Instrumente wie Gruppendiskussionen oder Planspiele vorsehen."@de .	

spv:ResMethPrototyping a owl:NamedIndividual , spv:ResearchMethod ;
			schema:name "Prototyping (Wilde/Hess)"@en ;
			schema:name "Prototyping (Wilde/Hess)"@de ;
			schema:isBasedOn <http://doi.org/10.1007/s11576-007-0064-z> ;
			rdfs:comment "Es wird eine Vorabversion eines Anwendungssystems entwickelt und evaluiert. Beide Schritte können neue Erkenntnisse generieren."@de .	

spv:ResMethEthnography a owl:NamedIndividual , spv:ResearchMethod ;
			schema:name "Ethnography (Wilde/Hess)"@en ;
			schema:name "Ethnographie (Wilde/Hess)"@de ;
			schema:isBasedOn <http://doi.org/10.1007/s11576-007-0064-z> ;
			rdfs:comment "Die Ethnographie möchte durch partizipierende Beobachtung Erkenntnisse generieren. Der Unterschied zur Fallstudie liegt in dem sehr hohen Umfang, in dem sich der Forscher in das untersuchte soziale Umfeld integriert. Eine objektive Distanz ist kaum vorhanden."@de .	

spv:ResMethCaseStudy a owl:NamedIndividual , spv:ResearchMethod ;
			schema:name "Case Study (Wilde/Hess)"@en ;
			schema:name "Fallstudie (Wilde/Hess)"@de ;
			schema:isBasedOn <http://doi.org/10.1007/s11576-007-0064-z> ;
			rdfs:comment "Die Fallstudie untersucht in der Regel komplexe, schwer abgrenzbare Pha¨nomene in ihrem natu¨rlichen Kontext. Sie stellt eine spezielle Form der qualitativ-empirischen Methodik dar, die wenige Merkmalsträger intensiv untersucht. Es steht entweder die möglichst objektive Untersuchung von Thesen (verhaltenswissenschaftlicher Zugang) oder die Interpretation von Verhaltensmustern als Phänotypen der von den Probanden konstruierten Realitäten (konstruktionsorientierter Zugang) im Mittelpunkt."@de .			

spv:ResMethGroundedTheory a owl:NamedIndividual , spv:ResearchMethod ;
			schema:name "Grounded Theory (Wilde/Hess)"@en ;
			schema:name "Grounded Theory (Wilde/Hess)"@de ;
			schema:isBasedOn <http://doi.org/10.1007/s11576-007-0064-z> ;
			rdfs:comment "Die Grounded Theory („gegenstandsverankerte Theoriebildung“) zielt auf die induktive Gewinnung neuer Theorien durch intensive Beobachtung des Untersuchungsgegenstandes im Feld. Die verschiedenen Vorgehensweisen zu Kodierung und Auswertung der vorwiegend qualitativen Daten sind exakt spezifiziert."@de .	

spv:ResMethQualitativeResearch a owl:NamedIndividual , spv:ResearchMethod ;
			schema:name "Qualitative Research (Wilde/Hess)"@en ;
			schema:name "Qualitative Querschnittsanalyse (Wilde/Hess)"@de ;
			schema:isBasedOn <http://doi.org/10.1007/s11576-007-0064-z> ;
			rdfs:comment "Diese Methode fasst Erhebungstechniken wie Fragebögen, Interviews, Delphi-Methode, Inhaltsanalysen etc. zu einem Aggregat zusammen. Sie umfasst eine einmalige Erhebung über mehrere Individuen hinweg, die anschließend qualitativ kodiert und ausgewertet wird. Ergebnis ist ein Querschnittsbild über die Stichprobenteilnehmer hinweg, welches üblicherweise Rückschlüsse auf die Grundgesamtheit zulässt."@de .	

spv:ResMethQuantitativeResearch a owl:NamedIndividual , spv:ResearchMethod ;
			schema:name "Quantitative Research (Wilde/Hess)"@en ;
			schema:name "Quantitative Querschnittsanalyse (Wilde/Hess)"@de ;
			schema:isBasedOn <http://doi.org/10.1007/s11576-007-0064-z> ;
			rdfs:comment "Diese Methode fasst Erhebungstechniken wie Fragebögen, Interviews, Delphi-Methode, Inhaltsanalysen etc. zu einem Aggregat zusammen. Sie umfasst eine einmalige Erhebung über mehrere Individuen hinweg, die anschließend quantitativ kodiert und ausgewertet wird. Ergebnis ist ein Querschnittsbild über die Stichprobenteilnehmer hinweg, welches üblicherweise Rückschlüsse auf die Grundgesamtheit zulässt."@de .	

spv:ResMethLabExperiment a owl:NamedIndividual , spv:ResearchMethod ;
			schema:name "Laboratory Experiment (Wilde/Hess)"@en ;
			schema:name "Laborexperiment (Wilde/Hess)"@de ;
			schema:isBasedOn <http://doi.org/10.1007/s11576-007-0064-z> ;
			rdfs:comment "Das Laborexperiment untersucht Kausalzusammenhänge in kontrollierter Umgebung, indem eine Experimentalvariable auf wiederholbare Weise manipuliert und die Wirkung der Manipulation gemessen wird. Der Untersuchungsgegenstand wird in künstlicher Umgebung (im „Labor“) untersucht, wodurch wesentlich die Möglichkeiten der Umgebungskontrolle beeinflusst werden."@de .	

spv:ResMethFieldExperiment a owl:NamedIndividual , spv:ResearchMethod ;
			schema:name "Field Experiment (Wilde/Hess)"@en ;
			schema:name "Feldexperiment (Wilde/Hess)"@de ;
			schema:isBasedOn <http://doi.org/10.1007/s11576-007-0064-z> ;
			rdfs:comment "Das Feldrexperiment untersucht Kausalzusammenhänge in kontrollierter Umgebung, indem eine Experimentalvariable auf wiederholbare Weise manipuliert und die Wirkung der Manipulation gemessen wird. Der Untersuchungsgegenstand wird in seiner natürlichen Umgebung (im „Feld“) untersucht, wodurch wesentlich die Möglichkeiten der Umgebungskontrolle beeinflusst werden."@de .	
			
spv:ResMethLiteratureAnalysis a owl:NamedIndividual , spv:ResearchMethod ;
			schema:name "Literature Analysis)"@en ;
			schema:name "Literaturanalyse"@de ;
			#schema:isBasedOn <http://doi.org/10.1007/s11576-007-0064-z> ;
			rdfs:comment " "@de .	
			

## Research Action Types ##
spv:ResActTypeDevelop a owl:NamedIndividual , spv:ResearchActionType ;
			rdfs:comment "Description" ;
			schema:name "develop"@en ;
			schema:name "entwickeln"@de .
			
spv:ResActTypeAnalyze a owl:NamedIndividual , spv:ResearchActionType ;
			rdfs:comment "Description" ;
			schema:name "analyze"@en ;
			schema:name "analysieren"@de .
			
spv:ResActTypeProve a owl:NamedIndividual , spv:ResearchActionType ;
			rdfs:comment "Description" ;
			schema:name "prove"@en ;
			schema:name "prüfen, erproben"@de .
			
spv:ResActTypeConceptualize a owl:NamedIndividual , spv:ResearchActionType ;
			rdfs:comment "Description" ;
			schema:name "conceptualize"@en ;
			schema:name "konzeptualisieren"@de .
			
spv:ResActTypeConstruct a owl:NamedIndividual , spv:ResearchActionType ;
			rdfs:comment "Description" ;
			schema:name "construct"@en ;
			schema:name "konstruieren"@de .

spv:ResActTypeEvaluate a owl:NamedIndividual , spv:ResearchActionType ;
			rdfs:comment "Description" ;
			schema:name "evaluate"@en ;
			schema:name "evaluieren"@de .
			
spv:ResActTypeElicit a owl:NamedIndividual , spv:ResearchActionType ;
			rdfs:comment "Description" ;
			schema:name "elicit"@en ;
			schema:name "erheben"@de .
			
spv:ResActTypeDesign a owl:NamedIndividual , spv:ResearchActionType ;
			rdfs:comment "Description" ;
			schema:name "design"@en ;
			schema:name "entwerfen/konzipieren"@de .
			
spv:ResActTypeStructure a owl:NamedIndividual , spv:ResearchActionType ;
			rdfs:comment "Description" ;
			schema:name "structure"@en ;
			schema:name "strukturieren"@de .
			
spv:ResActTypeCollect a owl:NamedIndividual , spv:ResearchActionType ;
			rdfs:comment "Description" ;
			schema:name "collect"@en ;
			schema:name "sammeln"@de .
			
spv:ResActTypeEnhance a owl:NamedIndividual , spv:ResearchActionType ;
			rdfs:comment "Description" ;
			schema:name "enhance"@en ;
			schema:name "verbessern"@de .

spv:ResActTypeExtract a owl:NamedIndividual , spv:ResearchActionType ;
			rdfs:comment "Description" ;
			schema:name "extract"@en ;
			schema:name "extrahieren"@de .

spv:ResActTypeProvide a owl:NamedIndividual , spv:ResearchActionType ;
			rdfs:comment "Description" ;
			schema:name "provide"@en ;
			schema:name "bereitstellen"@de .

spv:ResActTypeExtend a owl:NamedIndividual , spv:ResearchActionType ;
			rdfs:comment "Description" ;
			schema:name "extend"@en ;
			schema:name "erweitern"@de .

spv:ResActTypeImplement a owl:NamedIndividual , spv:ResearchActionType ;
			rdfs:comment "Description" ;
			schema:name "implement"@en ;
			schema:name "implementieren"@de .

spv:ResActTypeIntegrate a owl:NamedIndividual , spv:ResearchActionType ;
			rdfs:comment "Description" ;
			schema:name "integrate"@en ;
			schema:name "integrieren"@de .
			
spv:ResActTypeDefine a owl:NamedIndividual , spv:ResearchActionType ;
			rdfs:comment "Description" ;
			schema:name "define"@en ;
			schema:name "definieren"@de .
					

## Artifacts of Research and Development ##
spv:ResArtifactBlueprint a owl:NamedIndividual , spv:ResearchArtifact ;
			rdfs:comment "Description" ;
			schema:name "Blueprint"@en ;
			schema:name "Konzept"@de .

spv:ResArtifactRequirements a owl:NamedIndividual , spv:ResearchArtifact ;
			rdfs:comment "Description" ;
			schema:name "Requirements"@en ;
			schema:name "Anforderungen"@de .
			
spv:ResArtifactApplication a owl:NamedIndividual , spv:ResearchArtifact ;
			rdfs:comment "Description" ;
			schema:name "Application"@en ;
			schema:name "Anwendung"@de .
			
spv:ResArtifactSoftware a owl:NamedIndividual , spv:ResearchArtifact ;
			rdfs:comment "Description" ;
			schema:name "Software"@en ;
			schema:name "Software/ Programm"@de .
			
spv:ResArtifactHardware a owl:NamedIndividual , spv:ResearchArtifact ;
			rdfs:comment "Description" ;
			schema:name "Hardware"@en ;
			schema:name "Hardware"@de .
			
spv:ResArtifactSystem a owl:NamedIndividual , spv:ResearchArtifact ;
			rdfs:comment "Description" ;
			schema:name "System"@en ;
			schema:name "System"@de .
			
spv:ResArtifactITSystem a owl:NamedIndividual , spv:ResearchArtifact ;
			rdfs:comment "Description" ;
			schema:name "IT System"@en ;
			schema:name "IT-System"@de .
			
spv:ResArtifactProcess a owl:NamedIndividual , spv:ResearchArtifact ;
			rdfs:comment "Description" ;
			schema:name "Process"@en ;
			schema:name "Prozess"@de .
			
spv:ResArtifactBusinessProcess a owl:NamedIndividual , spv:ResearchArtifact ;
			rdfs:comment "Description" ;
			schema:name "Business Process"@en ;
			schema:name "Geschäftsprozess"@de .
			
spv:ResArtifactMethod a owl:NamedIndividual , spv:ResearchArtifact ;
			rdfs:comment "Description" ;
			schema:name "Method"@en ;
			schema:name "Method"@de .

spv:ResArtifactFramework a owl:NamedIndividual , spv:ResearchArtifact ;
			rdfs:comment "Description" ;
			schema:name "Framework"@en ;
			schema:name "Framework/ Rahmenwerk"@de .

spv:ResArtifactPolicy a owl:NamedIndividual , spv:ResearchArtifact ;
			rdfs:comment "Description" ;
			schema:name "Policy"@en ;
			schema:name "Leitlinie"@de .

spv:ResArtifactStandard a owl:NamedIndividual , spv:ResearchArtifact ;
			rdfs:comment "Description" ;
			schema:name "Standard, Guidline"@en ;
			schema:name "Richtlinie"@de .

spv:ResArtifactNLPArtifact a owl:NamedIndividual , spv:ResearchArtifact ;
			rdfs:comment "Element, Baustein der Verarbeitung natürlicher Sprache, z. B. Schlüsselphrasen, Schlüssel- und Stopwortlisten" ;
			schema:name "NLP Artifact"@en ;
			schema:name "NLP Artefakt"@de .
			
spv:ResArtifactOntology a owl:NamedIndividual , spv:ResearchArtifact ;
			rdfs:comment "semantische Netze unterschiedlicher Ausbaustufe; bis zu formal spezifizierten Konzeptualisierungen einer Domäne" ;
			schema:name "Ontology"@en ;
			schema:name "Ontologie"@de .
						
spv:ResArtifactLinkedData a owl:NamedIndividual , spv:ResearchArtifact ;
			rdfs:comment "" ;
			schema:name "Linked Data"@en ;
			schema:name "Linked Data"@de .
			
spv:ResArtifactWorkflow a owl:NamedIndividual , spv:ResearchArtifact ;
			rdfs:comment "" ;
			schema:name "Workflow"@en ;
			schema:name "Workflow"@de .			

spv:ResArtifactTermDefinition a owl:NamedIndividual , spv:ResearchArtifact ;
			rdfs:comment "" ;
			schema:name "Term Definition"@en ;
			schema:name "Begriffsdefinition"@de .			

spv:ResArtifactModelingLanguage a owl:NamedIndividual , spv:ResearchArtifact ;
			rdfs:comment "" ;
			schema:name "Modeling Language"@en ;
			schema:name "Modellierungssprache"@de .			

spv:ResArtifactDevFramework a owl:NamedIndividual , spv:ResearchArtifact ;
			rdfs:comment "" ;
			schema:name "Development Framework"@en ;
			schema:name "Entwicklungsumgebung"@de .			

spv:ResArtifactDevDocumentation a owl:NamedIndividual , spv:ResearchArtifact ;
			rdfs:comment "" ;
			schema:name "Documentation"@en ;
			schema:name "Dokumentation"@de .			
